fixing patterns to be more sensible.

examples/mtac/McMtac.v
@@ -11,11 +11,19 @@
  **)
 Require Import ExtLib.Core.RelDec.
 Require Import ExtLib.Structures.Monads.
+Require Import ExtLib.Structures.Traversable.
 Require Import ExtLib.Data.List.
 Require Import ExtLib.Data.Monads.ReaderMonad.
 Require Import ExtLib.Data.Vector.
 Require Import MirrorCore.Ext.Expr.
 Require Import MirrorCore.Ext.ExprUnifySyntactic.
+Require MirrorCore.SealedSubst.
+
+(** This is just a default. Most users won't want/want
+ ** to chnage this, but if there is a better substitution
+ ** available we should change to use that.
+ **)
+Require MirrorCore.Ext.FMapSubst.
 
 Set Implicit Arguments.
 Set Strict Implicit.
@@ -27,42 +35,101 @@ Record McEnv : Type :=
 ; mtac_fuel : nat
 }.
 
-Definition McMtac := reader McEnv.
+Definition McMtacT := readerT McEnv.
 
-Definition runMcMtac {T} (fs : tfunctions) (tus tvs : EnvI.tenv typ)
-           (fuel : nat) (cmd : McMtac T) : T :=
-  runReader cmd {| mtac_tfuncs := fs
-                 ; mtac_tus := tus
-                 ; mtac_tvs := tvs
-                 ; mtac_fuel := fuel |}.
+Definition runMcMtac {T} {m : Type -> Type} (fs : tfunctions) (tus tvs : EnvI.tenv typ)
+           (fuel : nat) (cmd : McMtacT m T) : m T :=
+  runReaderT cmd {| mtac_tfuncs := fs
+                  ; mtac_tus := tus
+                  ; mtac_tvs := tvs
+                  ; mtac_fuel := fuel |}.
 
-Global Instance Monad_McMtac : Monad McMtac := _.
-Instance MonadReader_McMtac : MonadReader McEnv McMtac := _.
+Global Instance Monad_McMtac m (M : Monad m) : Monad (McMtacT m) := _.
+Instance MonadReader_McMtac m (M : Monad m) : MonadReader McEnv (McMtacT m) := _.
+Global Instance MonadT_McMtac m (M : Monad m) : MonadT (McMtacT m) m := _.
 
-Definition mc_expr (t : Type) : Type := expr.
+Definition mc_expr (t : typ) : Type := expr.
 
-Definition mpattern := expr.
+Inductive mpattern :=
+| PGet (i : nat) (t : typ)
+| PVar (v : nat)
+| PUVar (u : uvar)
+| PFunc (f : func) (ls : list typ)
+| PApp (l r : mpattern)
+| PAbs (t : typ) (e : mpattern)
+| PEqual (t : typ) (l r : mpattern)
+| PNot (e : mpattern).
 
-Definition omax (l r : option nat) : option nat :=
-  match l , r with
-    | Some l , Some r => Some (max l r)
-    | None , r => r
-    | l , None => l
-  end.
-
-Fixpoint vars_of_mpattern (p : mpattern) : option nat :=
+Fixpoint typeof_mpattern (tfs : tfunctions) (tus tvs : list typ) (p : mpattern)
+: option typ :=
   match p with
-    | Var _
-    | Func _ _ => None
-    | App l r => omax (vars_of_mpattern l) (vars_of_mpattern r)
-    | Abs _ e => vars_of_mpattern e
-    | UVar u => Some u
-    | Equal _ l r => omax (vars_of_mpattern l) (vars_of_mpattern r)
-    | Not e => vars_of_mpattern e
+    | PGet _ t => Some t
+    | PVar v => nth_error tvs v
+    | PUVar u => nth_error tus u
+    | PFunc f ts =>
+      match nth_error tfs f with
+        | Some r =>
+          if EqNat.beq_nat (length ts) (tfenv r)
+          then Some (instantiate_typ ts (tftype r))
+          else None
+        | None => None
+      end
+    | PApp l r =>
+      bind (typeof_mpattern tfs tus tvs l)
+           (fun tf =>
+              bind (typeof_mpattern tfs tus tvs r) (type_of_apply tf))
+    | PAbs t e =>
+      bind (typeof_mpattern tfs tus (t :: tvs) e)
+           (fun t' => ret (tvArr t t'))
+    | PEqual t l r =>
+      bind (typeof_mpattern tfs tus tvs l)
+           (fun tl => bind (typeof_mpattern tfs tus tvs r)
+                           (fun tr => if andb (t ?[ eq ] tl) (t ?[ eq ] tr)
+                                      then Some tvProp else None))
+    | PNot e =>
+      bind (typeof_mpattern tfs tus tvs e)
+           (fun tl => if tl ?[ eq ] tvProp then Some tvProp else None)
   end.
+
+Definition expr_of_mpattern (Ubase : uvar) : mpattern -> expr :=
+  fix recur (p : mpattern) : expr :=
+  match p with
+    | PGet u _ => UVar (Ubase + u)
+    | PVar v => Var v
+    | PUVar v => UVar v
+    | PFunc f ts => Func f ts
+    | PApp l r => App (recur l) (recur r)
+    | PAbs t e => Abs t (recur e)
+    | PEqual t l r => Equal t (recur l) (recur r)
+    | PNot e => Not (recur e)
+  end.
+
+Fixpoint list_set (n : nat) (t : typ) (ls : list (option typ))
+: list (option typ) :=
+  match n with
+    | 0 => Some t :: tl ls
+    | S n => match ls with
+               | nil => None :: list_set n t nil
+               | t' :: ts => t' :: list_set n t ts
+             end
+  end.
+
+Fixpoint getEnv (p : mpattern) (ls : list (option typ)) : list (option typ) :=
+  match p with
+    | PGet u t => list_set u t ls
+    | PVar _ => ls
+    | PFunc _ _ => ls
+    | PApp l r => getEnv l (getEnv r ls)
+    | PAbs _ e => getEnv e ls
+    | PUVar _ => ls
+    | PEqual _ l r => getEnv l (getEnv r ls)
+    | PNot e => getEnv e ls
+  end.
+
+Definition binders_of_mpattern (ptrn : mpattern) : option (list typ) :=
+  mapT (fun x => x) (getEnv ptrn nil).
 
 Section exp_app.
-
   Variables D R : Type.
 
   Fixpoint exp n : Type :=
@@ -107,9 +174,6 @@ Definition lift_uvars (us uadd : nat) (e : expr) : expr :=
     | _ => lift_uvars' us uadd e
   end.
 
-Require MirrorCore.SealedSubst.
-Require MirrorCore.Ext.FMapSubst.
-
 Definition subst := SealedSubst.seal_subst FMapSubst.SUBST.subst.
 Local Instance Subst_subst : Subst.Subst subst expr :=
   @SealedSubst.Subst_seal_subst _ _ FMapSubst.SUBST.Subst_subst.
@@ -130,131 +194,149 @@ Fixpoint get_args_from (sub : subst) from cnt : option (vector expr cnt) :=
       end
   end.
 
-Inductive Branch (T : Type) : Type :=
-| Case (p : mpattern) (d : match vars_of_mpattern p with
-                             | None => McMtac T
-                             | Some p => exp expr (McMtac T) (S p)
-                           end).
+Section over_monad.
+  Variable m : Type -> Type.
+  Variable Monad_m : Monad m.
 
-Definition typeof (t : expr) : McMtac (option typ) :=
-  bind (Monad := Monad_McMtac) ask (fun env =>
-              let tf := env.(mtac_tfuncs) in
-              let tus := env.(mtac_tus) in
-              let tvs := env.(mtac_tvs) in
-              let fuel := env.(mtac_fuel) in
-              ret (typeof_expr tf tus tvs t)).
+  (** Typeof **)
+  Definition typeof (t : expr) : McMtacT m (option typ) :=
+    bind (Monad := Monad_McMtac Monad_m) ask (fun env =>
+      let tf := env.(mtac_tfuncs) in
+      let tus := env.(mtac_tus) in
+      let tvs := env.(mtac_tvs) in
+      let fuel := env.(mtac_fuel) in
+      ret (typeof_expr tf tus tvs t)).
 
-Definition _mmatchAt {T}
-           (e: expr) (ty : typ)
-           (ls : list (Branch T))
-           (default : McMtac T) : McMtac T :=
-  bind (Monad := Monad_McMtac) ask (fun env =>
-              let tf := env.(mtac_tfuncs) in
-              let tus := env.(mtac_tus) in
-              let tvs := env.(mtac_tvs) in
-              let fuel := env.(mtac_fuel) in
-              (fix find_pattern (pats : list (Branch T))  : McMtac T :=
-                 match pats with
-                   | nil => default
-                   | Case p case :: ps =>
-                     let p' := lift_uvars (length tus) (length tus) p in
-                     match
-                       @exprUnify subst _ tf fuel tus tvs 0
-                                  (empty_above (length tus))
-                                  e p' ty
-                     with
-                       | None => find_pattern ps
-                       | Some sub =>
-                         match vars_of_mpattern p as vs
-                           return match vs with
-                                    | None => McMtac T
-                                    | Some p => exp expr (McMtac T) (S p)
-                                  end -> McMtac T
-                         with
-                           | None => fun x => x
-                           | Some var_count => fun case =>
-                             match
-                               get_args_from sub (length tus) (S var_count)
-                             with
-                               | Some args =>
-                                 @exp_app_vector _ (McMtac T) (S var_count) args case
-                               | None => find_pattern ps
-                             end
-                         end case
-                     end
-                 end) ls).
+  (** Pattern matching **)
+  Context {T : Type}.
 
-Definition _mmatch {T}
-           (t : expr)
-           (ls : list (Branch T))
-           (default : McMtac T) : McMtac T :=
-  bind (Monad := Monad_McMtac) ask (fun env =>
-              let tf := env.(mtac_tfuncs) in
-              let tus := env.(mtac_tus) in
-              let tvs := env.(mtac_tvs) in
-              let fuel := env.(mtac_fuel) in
-              match typeof_expr tf tus tvs t with
-                | None => default
-                | Some ty =>
-                  (fix find_pattern (pats : list (Branch T))  : McMtac T :=
-                     match pats with
-                       | nil => default
-                       | Case p case :: ps =>
-                         let p' := lift_uvars (length tus) (length tus) p in
-                         match
-                           @exprUnify subst _ tf fuel tus tvs 0
-                                      (empty_above (length tus))
-                                      t p' ty
-                         with
-                           | None => find_pattern ps
-                           | Some sub =>
-                             match vars_of_mpattern p as vs
-                                   return match vs with
-                                            | None => McMtac T
-                                            | Some p => exp expr (McMtac T) (S p)
-                                          end -> McMtac T
-                             with
-                               | None => fun x => x
-                               | Some var_count => fun case =>
-                                 match
-                                   get_args_from sub (length tus) (S var_count)
-                                 with
-                                   | Some args =>
-                                     @exp_app_vector _ (McMtac T) (S var_count) args case
-                                   | None => find_pattern ps
-                                 end
-                             end case
-                         end
-                     end) ls
-              end).
+  Fixpoint arm_result (ls : list typ) : Type :=
+    match ls with
+      | nil => McMtacT m T
+      | l :: ls => mc_expr l -> arm_result ls
+    end.
+
+  Inductive Branch : Type :=
+  | Case (p : mpattern) (d : match binders_of_mpattern p with
+                               | None => unit (** ill-typed pattern **)
+                               | Some p => arm_result p
+                             end).
+
+  Let arm_type :=
+    nat -> list typ -> list typ -> (unit -> McMtacT m T) -> expr -> typ -> McMtacT m T.
+
+  Definition arm_result_apply (s : subst) (error : unit -> McMtacT m T)
+  : nat -> forall ls : list typ, arm_result ls -> McMtacT m T :=
+    (fix recur (from : nat) (ls : list typ) : arm_result ls -> McMtacT m T :=
+       match ls with
+         | nil => fun x => x
+         | l :: ls => fun f =>
+                        match Subst.lookup from s with
+                          | None => error tt
+                          | Some e => recur (S from) ls (f e)
+                        end
+       end).
+
+  Definition BranchD (tfs : tfunctions) (a : Branch)
+  : arm_type :=
+    match a with
+      | Case p case =>
+        match binders_of_mpattern p as v
+          return match v with
+                   | None => unit
+                   | Some ps => arm_result ps
+                 end -> arm_type
+        with
+          | None => fun _ _ _ _ error _ _ => error tt
+          | Some pus => fun case fuel tus tvs error e ty =>
+            let count_tus := length tus in
+            let p' := expr_of_mpattern count_tus p in
+            match
+              @exprUnify subst _ tfs fuel (tus ++ pus) tvs 0
+                         (empty_above count_tus)
+                         e p' ty
+            with
+              | None => error tt
+              | Some sub =>
+                @arm_result_apply sub error count_tus
+                                 _ case
+            end
+        end case
+    end.
+
+  Definition _mmatchAt
+             (e: expr) (ty : typ)
+             (ls : list Branch)
+             (default : McMtacT m T) : McMtacT m T :=
+    bind (Monad := Monad_McMtac Monad_m) ask (fun env =>
+                let tf := env.(mtac_tfuncs) in
+                let tus := env.(mtac_tus) in
+                let tvs := env.(mtac_tvs) in
+                let fuel := env.(mtac_fuel) in
+                (fix find_pattern (pats : list Branch)  : McMtacT m T :=
+                   match pats with
+                     | nil => default
+                     | b :: ps =>
+                       BranchD tf b fuel tus tvs (fun t =>
+                                                    match t with
+                                                      | tt => find_pattern ps
+                                                    end) e ty
+                   end) ls).
+
+  Definition _mmatch
+             (e : expr)
+             (ls : list Branch)
+             (default : McMtacT m T) : McMtacT m T :=
+    bind (Monad := Monad_McMtac Monad_m) ask (fun env =>
+                let tf := env.(mtac_tfuncs) in
+                let tus := env.(mtac_tus) in
+                let tvs := env.(mtac_tvs) in
+                let fuel := env.(mtac_fuel) in
+                match typeof_expr tf tus tvs e with
+                  | None => default
+                  | Some ty =>
+                    (fix find_pattern (pats : list Branch)  : McMtacT m T :=
+                       match pats with
+                         | nil => default
+                         | b :: ps =>
+                           BranchD tf b fuel tus tvs (fun t =>
+                                                        match t with
+                                                          | tt => find_pattern ps
+                                                        end) e ty
+                       end) ls
+                end).
+End over_monad.
 
 Module McMtacNotation.
   Delimit Scope mcmtac_scope with mcmtac.
   Delimit Scope mcpattern_scope with mcmtac_pattern.
   Notation "[  x  ]  '=>>' e" :=
-    (@Case _ x e%mcmtac)
+    (@Case _ _ x e%mcmtac)
       (at level 50) : mcpattern_scope.
   Delimit Scope mcpatterns_scope with mcmtac_patterns.
   Notation "| p1 | .. | p2" :=
-    (@cons (@Branch _) p1%mcmtac_pattern ..
-           (@cons (@Branch _) p2%mcmtac_pattern nil) ..)
+    (@cons (@Branch _ _) p1%mcmtac_pattern ..
+           (@cons (@Branch _ _) p2%mcmtac_pattern nil) ..)
       (at level 50) : mcpatterns_scope.
   Notation "'mmatch' t 'with' ps \ e 'end'" :=
-    (@_mmatch _ t ps%mcmtac_patterns e%mcmtac) (at level 50) : mcmtac_scope.
+    (@_mmatch _ _ _ t ps%mcmtac_patterns e%mcmtac) (at level 50) : mcmtac_scope.
 
   Notation "'mmatch' t '@' ty 'with' ps \ e 'end'" :=
-    (@_mmatchAt _ t ty ps%mcmtac_patterns e%mcmtac) (at level 50) : mcmtac_scope.
+    (@_mmatchAt _ _ _ t ty ps%mcmtac_patterns e%mcmtac) (at level 50) : mcmtac_scope.
 
   (** Morally, this is just [e] **)
   Notation "'mmatch' t 'with' \ e 'end'" :=
-    (@_mmatch _ t nil e%mcmtac) (at level 50) : mcmtac_scope.
+    (@_mmatch _ _ _ t nil e%mcmtac) (at level 50) : mcmtac_scope.
+
+  Notation "'mmatch' t '@' ty 'with' \ e 'end'" :=
+    (@_mmatchAt _ _ _ t ty nil e%mcmtac) (at level 50) : mcmtac_scope.
 
 (*
-  Eval cbv iota in ([ Var 0 ] =>> ret true)%mcmtac_pattern.
-  Eval cbv iota in ([ UVar 0 ] =>> ret)%mcmtac_pattern.
+  Eval cbv iota in ([ PVar 0 ] =>> ret true)%mcmtac_pattern.
+  Eval cbv iota in ([ PGet 0 (tvType 0) ] =>> ret)%mcmtac_pattern.
 
   Eval cbv iota in (fun x => mmatch x with
-                               | [ UVar 0 ] =>> fun x => ret true
+                               | [ PGet 0 (tvType 0) ] =>> fun x => ret true
                                \ ret false
                              end)%mcmtac.
 
